Working on scheduling proof

src/hls/GiblePar.v
@@ -50,8 +50,8 @@ Module ParBB <: BlockType.
 
     Context {A B: Type} (ge: Genv.t A B).
 
-    Definition step_instr_list := step_list (step_instr ge).
-    Definition step_instr_seq := step_list step_instr_list.
+    Definition step_instr_list := step_list_inter (step_instr ge).
+    Definition step_instr_seq := step_list_inter step_instr_list.
     Definition step_instr_block := step_list step_instr_seq.
 
 (*|
